stash experiments

tests/lean/run/pord.lean
@@ -47,12 +47,53 @@ instance instPOrdT : (xs : T) → (ys : T) → @POrd T xs ys
 def instPOrd_of_ord {α} [Ord α] (x y : α) : @POrd α x y := ⟨Ord.compare x y⟩
 -- def instOrd_of_pord {α} [∀ (x y : α), POrd x y] : @Ord α := ⟨fun x y => POrd.pord x y⟩
 
-attribute [local instance] instPOrd_of_ord in
-instance [Ord α] : Ord (List α) where
-  compare x y := POrd.pord x y
+-- attribute [local instance] instPOrd_of_ord in
+-- instance [Ord α] : Ord (List α) where
+  -- compare x y := POrd.pord x y
 
 instance : Ord T where
   compare x y := POrd.pord x y
 
 theorem T.ordSpec : compare (T.node xs) (T.node ys) = compare xs ys := by
   simp [compare, POrd.pord, instPOrdT]
+
+attribute [instance] List.instOrd
+
+def List.compare_of_compare : ∀ (xs ys : List α), (compare : ∀ x y, x ∈ xs → y ∈ ys → Ordering) →
+    Ordering
+  | [], [], _ => .eq
+  | [], _::__, _ => .lt
+  | _::_, [], _ => .gt
+  | x::xs, y::ys, f =>
+    (f x y List.mem_cons_self List.mem_cons_self).then
+      (List.compare_of_compare xs ys (fun x y hx hy => f x y (List.mem_cons_of_mem _ hx) (List.mem_cons_of_mem _ hy)))
+
+@[wf_preprocess]
+theorem List.instOrd_compare_wfParam (i : Ord α) : ∀ (xs ys : List α),
+   (@List.instOrd _ i).compare (wfParam xs) ys =
+    List.compare_of_compare xs ys (fun x y _ _ => i.compare x y) := by
+  intros xs ys
+  induction xs generalizing ys
+  · cases ys
+    · simp [Ord.compare, List.compareLex, wfParam, List.compare_of_compare]
+    · simp [Ord.compare, List.compareLex, wfParam, List.compare_of_compare]
+  · cases ys
+    · simp [Ord.compare, List.compareLex, wfParam, List.compare_of_compare]
+    · simp [Ord.compare, List.compareLex, wfParam, List.compare_of_compare, *]
+      split <;> simp_all
+      sorry
+
+@[wf_preprocess]
+theorem Ord.compare_mk {f : α → α → Ordering} : @Ord.compare _ (Ord.mk f) = f := rfl
+
+-- @[wf_preprocess]
+-- theorem Ord.compare_mk' {f : α → α → Ordering} : @Ord.compare _ (Ord.mk f) x y = f x y := rfl
+
+-- Why does it not beta-reduce here?
+
+set_option trace.Elab.definition.wf true in
+def T.compare : (xs : T) → (ys : T) → Ordering
+  | .node xs, .node ys =>
+    letI : Ord T := ⟨T.compare⟩
+    Ord.compare xs ys
+termination_by xs => xs
